list now works

src/ENVCAP/Core/TypeChecker.hs
@@ -5,6 +5,7 @@
 {-# HLINT ignore "Use >=>" #-}
 module ENVCAP.Core.TypeChecker where
 
+import Debug.Trace (trace)
 import ENVCAP.Syntax
 
 data TypeError = TypeError String deriving (Eq, Show)
@@ -37,10 +38,10 @@ isLabel _ _ = False
 -- True
 containment :: CoreTyp -> CoreTyp -> Bool
 containment (TyCRecord l tA) (TyCRecord label typ) =
-    l == label && tA == typ
+  l == label && tA == typ
 containment (TyCRecord l tA) (TyCAnd tB tC) =
-    (containment (TyCRecord l tA) tB && not (isLabel l tC))
-        || (containment (TyCRecord l tA) tC && not (isLabel l tB))
+  (containment (TyCRecord l tA) tB && not (isLabel l tC))
+    || (containment (TyCRecord l tA) tC && not (isLabel l tB))
 containment _ _ = False
 
 -- `containmentUnion` checks if the record type is contained in the union type.
@@ -51,10 +52,10 @@ containment _ _ = False
 -- True
 containmentUnion :: CoreTyp -> CoreTyp -> Bool
 containmentUnion (TyCRecord l tA) (TyCRecord label typ) =
-    l == label && tA == typ
+  l == label && tA == typ
 containmentUnion (TyCRecord l tA) (TyCUnion tB tC) =
-    (containmentUnion (TyCRecord l tA) tB && not (isLabel l tC))
-        || (containmentUnion (TyCRecord l tA) tC && not (isLabel l tB))
+  (containmentUnion (TyCRecord l tA) tB && not (isLabel l tC))
+    || (containmentUnion (TyCRecord l tA) tC && not (isLabel l tB))
 containmentUnion _ _ = False
 
 -- `rlookupt` performs a look on the typing context by record
@@ -64,144 +65,140 @@ containmentUnion _ _ = False
 -- Just TyCInt
 rlookupt :: CoreTyp -> String -> Maybe CoreTyp
 rlookupt (TyCRecord l t) label
-    | l == label = Just t
+  | l == label = Just t
 rlookupt (TyCAnd tA tB) label =
-    case rlookupt tB label of
-        Just t -> Just t
-        Nothing -> rlookupt tA label
+  case rlookupt tB label of
+    Just t -> Just t
+    Nothing -> rlookupt tA label
 rlookupt _ _ = Nothing
 
-{- | `countLabels` is a utility function that ensures well-formedness of the variant type
-  and returns the count of labels present in the variant type.
-
-=== Example:
->>> countLabels (TyCRecord "x" TyInt)
-Right 1
--}
+-- | `countLabels` is a utility function that ensures well-formedness of the variant type
+--  and returns the count of labels present in the variant type.
+--
+-- === Example:
+-- >>> countLabels (TyCRecord "x" TyInt)
+-- Right 1
 countLabels :: CoreTyp -> Either TypeError Int
 countLabels (TyCRecord _ _) = Right 1
 countLabels (TyCUnion tA tB) =
-    do
-        left <- countLabels tA
-        right <- countLabels tB
-        return $ left + right
+  do
+    left <- countLabels tA
+    right <- countLabels tB
+    return $ left + right
 countLabels _ =
-    Left $ TypeError "Variant Type must be restricted to only records with unions"
+  Left $ TypeError "Variant Type must be restricted to only records with unions"
 
-{- | `countTypesInConstructor` is a utility function that returns the count of types
-inside an intersection type.
-
-=== Example:
->>> countTypesInConstructor (TyCAnd TyCInt TyCInt)
-Right 2
--}
+-- | `countTypesInConstructor` is a utility function that returns the count of types
+-- inside an intersection type.
+--
+-- === Example:
+-- >>> countTypesInConstructor (TyCAnd TyCInt TyCInt)
+-- Right 2
 countTypesInConstructor :: CoreTyp -> Either TypeError Int
 countTypesInConstructor (TyCAnd tA _) =
-    countTypesInConstructor tA >>= \left -> return $ left + 1
+  countTypesInConstructor tA >>= \left -> return $ left + 1
 countTypesInConstructor _ =
-    Right 1
+  Right 1
 
-{- | `isPatternPresentInVariantTy` is a utility function that ensures each case in a match statement
-  is well typed and returns the corresponding type of constructor from the variant type
-  via a type label lookup.
-
-=== Example:
->>> isPatternPresentInVariantTy (TyCUnion (TyCRecord "Num" TyCInt) (TyCRecord "Var" TyCString)) ("Var", ["x"])
-Right TyCString
-
->>> isPatternPresentInVariantTy (TyCUnion (TyCRecord "Num" TyCInt) (TyCRecord "Var" TyCString)) ("Var", ["x", "y"])
-Left (TypeError "The number of bindings in the case Var do not match the data type constructor")
-
->>> isPatternPresentInVariantTy (TyCUnion (TyCRecord "Num" TyCUnit) (TyCRecord "Var" TyCString)) ("Num", [])
-Right TyCUnit
--}
+-- | `isPatternPresentInVariantTy` is a utility function that ensures each case in a match statement
+--  is well typed and returns the corresponding type of constructor from the variant type
+--  via a type label lookup.
+--
+-- === Example:
+-- >>> isPatternPresentInVariantTy (TyCUnion (TyCRecord "Num" TyCInt) (TyCRecord "Var" TyCString)) ("Var", ["x"])
+-- Right TyCString
+--
+-- >>> isPatternPresentInVariantTy (TyCUnion (TyCRecord "Num" TyCInt) (TyCRecord "Var" TyCString)) ("Var", ["x", "y"])
+-- Left (TypeError "The number of bindings in the case Var do not match the data type constructor")
+--
+-- >>> isPatternPresentInVariantTy (TyCUnion (TyCRecord "Num" TyCUnit) (TyCRecord "Var" TyCString)) ("Num", [])
+-- Right TyCUnit
 isPatternPresentInVariantTy :: CoreTyp -> Pattern -> Either TypeError CoreTyp
 isPatternPresentInVariantTy variantTy (label, bindings) =
-    -- Firstly, a label lookup is performed on the variantTy
-    case rlookupVariant variantTy of
-        Just ty ->
-            -- This gives the type, but we need to ensure containment for uniqueness
-            if containmentUnion (TyCRecord label ty) variantTy
-                then
-                    if (ty == TyCUnit && countBindings == 0)
-                        || (countTypesInConstructor ty == Right countBindings)
-                        then Right ty
-                        else Left $ TypeError ("The number of bindings in the case " ++ label ++ " do not match the data type constructor")
-                else Left $ TypeError ("Duplicate constructor found in the variant type: " ++ show variantTy)
-        Nothing ->
-            Left $ TypeError ("Constructor " ++ label ++ " not present in the variant type: " ++ show variantTy)
+  -- Firstly, a label lookup is performed on the variantTy
+  case rlookupVariant variantTy of
+    Just ty ->
+      -- This gives the type, but we need to ensure containment for uniqueness
+      if containmentUnion (TyCRecord label ty) variantTy
+        then
+          if (ty == TyCUnit && countBindings == 0)
+            || (countTypesInConstructor ty == Right countBindings)
+            then Right ty
+            else Left $ TypeError ("The number of bindings in the case " ++ label ++ " do not match the data type constructor")
+        else Left $ TypeError ("Duplicate constructor found in the variant type: " ++ show variantTy)
+    Nothing ->
+      Left $ TypeError ("Constructor " ++ label ++ " not present in the variant type: " ++ show variantTy)
   where
     countBindings = length bindings
     rlookupVariant :: CoreTyp -> Maybe CoreTyp
     rlookupVariant (TyCRecord l t)
-        | l == label = Just t
+      | l == label = Just t
     rlookupVariant (TyCUnion tA tB) =
-        case rlookupVariant tB of
-            Just t -> Just t
-            Nothing -> rlookupVariant tA
+      case rlookupVariant tB of
+        Just t -> Just t
+        Nothing -> rlookupVariant tA
     rlookupVariant _ = Nothing
 
-{- | `insertIntersectionContext` is a utility function that inserts an intersection type in the context
-correct.
-
-=== Example:
->>> insertIntersectionContext (TyCAnd TyCUnit TyCInt) (TyCAnd (TyCAnd TyCString TyCInt) TyCBool)
-Right (TyCAnd (TyCAnd (TyCAnd (TyCAnd TyCUnit TyCInt) TyCString) TyCInt) TyCBool)
--}
+-- | `insertIntersectionContext` is a utility function that inserts an intersection type in the context
+-- correct.
+--
+-- === Example:
+-- >>> insertIntersectionContext (TyCAnd TyCUnit TyCInt) (TyCAnd (TyCAnd TyCString TyCInt) TyCBool)
+-- Right (TyCAnd (TyCAnd (TyCAnd (TyCAnd TyCUnit TyCInt) TyCString) TyCInt) TyCBool)
 insertIntersectionContext :: CoreTyp -> CoreTyp -> Either TypeError CoreTyp
 insertIntersectionContext ctx (TyCAnd tA tB) =
-    insertIntersectionContext ctx tA >>= \left -> return $ TyCAnd left tB
+  insertIntersectionContext ctx tA >>= \left -> return $ TyCAnd left tB
 insertIntersectionContext ctx ty =
-    Right $ TyCAnd ctx ty
+  Right $ TyCAnd ctx ty
 
 inferCase :: CoreTyp -> CoreTyp -> (Pattern, CoreTm) -> Either TypeError CoreTyp
 inferCase ctx variantTy ((label, bindings), tm) =
-    isPatternPresentInVariantTy variantTy (label, bindings) >>= \ty' ->
-        insertIntersectionContext ctx ty' >>= \ctx' ->
-            case infer ctx' tm of
-                Right caseTy ->
-                    Right caseTy
-                Left err -> Left err
+  isPatternPresentInVariantTy variantTy (label, bindings) >>= \ty' ->
+    insertIntersectionContext ctx ty' >>= \ctx' ->
+      case infer ctx' tm of
+        Right caseTy ->
+          Right caseTy
+        Left err -> Left err
 
 checkCases :: CoreTyp -> CoreTyp -> CoreTyp -> [(Pattern, CoreTm)] -> Either TypeError CoreTyp
 checkCases _ ty _ [] = Right ty
 checkCases ctx ty1 variantTy (x : xs) =
-    if checkEach (x : xs)
-        then Right ty1
-        else
-            Left $ TypeError "Types of each case don't match. Elaboration not sound."
+  if checkEach (x : xs)
+    then Right ty1
+    else
+      Left $ TypeError "Types of each case don't match. Elaboration not sound."
   where
     checkEach [] = True
     checkEach (fstcase : rest) =
-        case inferCase ctx variantTy fstcase of
-            Right ty' -> ty1 == ty' && checkEach rest
-            Left _ -> False
+      case inferCase ctx variantTy fstcase of
+        Right ty' -> ty1 == ty' && checkEach rest
+        Left _ -> False
 
 inferMatch :: CoreTyp -> CoreTm -> Either TypeError CoreTyp
 inferMatch _ (Case _ []) =
-    Left $ TypeError "Match statement must have atleast one case. Elaboration is not sound."
+  Left $ TypeError "Match statement must have atleast one case. Elaboration is not sound."
 inferMatch ctx (Case tm (fstcase : cases)) =
-    case infer ctx tm of
-        Right variantTy@(TyCUnion _ _) ->
-            if countLabels variantTy == Right (length cases + 1) && isUnique (fstcase : cases)
-                then
-                    inferCase ctx variantTy fstcase >>= \ty1 ->
-                        checkCases ctx ty1 variantTy cases
-                else Left $ TypeError "Fewer cases present in the match than the constructors in the ADT."
-        Right _ -> Left $ TypeError "match can only be called on variant"
-        Left err -> Left err
+  case infer ctx tm of
+    Right variantTy@(TyCUnion _ _) ->
+      if countLabels variantTy == Right (length cases + 1) && isUnique (fstcase : cases)
+        then
+          inferCase ctx variantTy fstcase >>= \ty1 ->
+            checkCases ctx ty1 variantTy cases
+        else Left $ TypeError "Fewer cases present in the match than the constructors in the ADT."
+    Right _ -> Left $ TypeError "match can only be called on variant"
+    Left err -> Left err
   where
     isUnique ls = case ls of
-        ((constructor, _), _) : xs ->
-            notFound constructor xs && isUnique xs
-        [] -> True
+      ((constructor, _), _) : xs ->
+        notFound constructor xs && isUnique xs
+      [] -> True
       where
         notFound l ls' = case ls' of
-            ((constructor', _), _) : xs ->
-                l /= constructor' && notFound l xs
-            [] -> True
+          ((constructor', _), _) : xs ->
+            l /= constructor' && notFound l xs
+          [] -> True
 inferMatch _ _ =
-    Left $ TypeError ""
+  Left $ TypeError ""
 
 -- `infer` infers the type of the expression.
 --
@@ -216,113 +213,117 @@ infer _ (EBool _) = Right TyCBool
 infer _ (EString _) = Right TyCString
 infer ctx (Lam tA e) = infer (TyCAnd ctx tA) e >>= \tB -> Right (TyCArrow tA tB)
 infer ctx (Proj e n) =
-    infer ctx e >>= \tB ->
-        case lookupt tB n of
-            Just t -> Right t
-            Nothing ->
-                Left $
-                    TypeError $
-                        "Projection "
-                            ++ show n
-                            ++ " failed on type "
-                            ++ show tB
-                            ++ " ctx: "
-                            ++ show ctx
+  infer ctx e >>= \tB ->
+    case lookupt tB n of
+      Just t -> Right t
+      Nothing ->
+        Left $
+          TypeError $
+            "Projection "
+              ++ show n
+              ++ " failed on type "
+              ++ show tB
+              ++ " ctx: "
+              ++ show ctx
 infer ctx (Clos e1 (Lam tA e2)) =
-    infer ctx e1 >>= \ctx1 ->
-        infer (TyCAnd ctx1 tA) e2 >>= \tB ->
-            Right (TyCArrow tA tB)
+  infer ctx e1 >>= \ctx1 ->
+    infer (TyCAnd ctx1 tA) e2 >>= \tB ->
+      Right (TyCArrow tA tB)
 infer ctx (Rec l e) = infer ctx e >>= \tA -> Right (TyCRecord l tA)
 infer ctx (RProj e l) =
-    infer ctx e >>= \tB ->
-        case rlookupt tB l of
-            Just tA ->
-                if containment (TyCRecord l tA) tB
-                    then Right tA
-                    else Left $ TypeError "Record projection failed due to containment"
-            Nothing -> Left $ TypeError $ "Field " ++ show l ++ " not found in type " ++ show tB
+  infer ctx e >>= \tB ->
+    case rlookupt tB l of
+      Just tA ->
+        if containment (TyCRecord l tA) tB
+          then Right tA
+          else Left $ TypeError "Record projection failed due to containment"
+      Nothing -> Left $ TypeError $ "Field " ++ show l ++ " not found in type " ++ show tB
 infer ctx (Box e1 e2) = infer ctx e1 >>= \ctx1 -> infer ctx1 e2
 infer ctx (Mrg e1 e2) = infer ctx e1 >>= \tA -> infer (TyCAnd ctx tA) e2 >>= \tB -> Right (TyCAnd tA tB)
 infer ctx (App e1 e2) =
-    infer ctx e1 >>= \ty1 ->
-        case ty1 of
-            TyCArrow tA tB ->
-                if check ctx e2 tA
-                    then Right tB
-                    else Left $ TypeError ("Type mismatch in application: Context:" ++ show ctx)
-            _ ->
-                Left $
-                    TypeError
-                        ( "Expected a function type in application Function Type: "
-                            ++ show ty1
-                            ++ " Function: "
-                            ++ show e1
-                        )
+  infer ctx e1 >>= \ty1 ->
+    case ty1 of
+      TyCArrow tA tB ->
+        if check ctx e2 tA
+          then Right tB
+          else Left $ TypeError ("Type mismatch in application: Context:" ++ show ctx)
+      _ ->
+        Left $
+          TypeError
+            ( "Expected a function type in application Function Type: "
+                ++ show ty1
+                ++ " Function: "
+                ++ show e1
+            )
 infer ctx (If cond e1 e2) =
-    if check ctx cond TyCBool
-        then
-            infer ctx e1 >>= \t1 ->
-                infer ctx e2 >>= \t2 ->
-                    if t1 == t2
-                        then Right t1
-                        else Left $ TypeError "Branches of if must have the same type"
-        else Left $ TypeError "Condition must be of type Bool"
+  if check ctx cond TyCBool
+    then
+      infer ctx e1 >>= \t1 ->
+        infer ctx e2 >>= \t2 ->
+          if t1 == t2
+            then Right t1
+            else Left $ TypeError "Branches of if must have the same type"
+    else Left $ TypeError "Condition must be of type Bool"
 infer ctx (Fix tA e) =
-    if check (TyCAnd ctx tA) e tA
-        then Right tA
-        else Left $ TypeError "Fixpoint type check failed"
+  if check (TyCAnd ctx tA) e tA
+    then Right tA
+    else Left $ TypeError "Fixpoint type check failed"
 infer ctx (Tag tm ty) = case infer ctx tm of
-    Right tm'@(TyCRecord _ _) ->
-        if containmentUnion tm' ty
-            then Right ty
-            else Left $ TypeError ("Ambiguous label on ADT. Elaboration FAILED. " ++ show (Tag tm ty))
-    Right _ -> Left $ TypeError "Value can't be tagged with ADT"
-    Left _ -> Left $ TypeError "Elaboration Failed"
+  Right tm'@(TyCRecord _ _) ->
+    if containmentUnion tm' ty
+      then Right ty
+      else Left $ TypeError ("Ambiguous label on ADT. Elaboration FAILED. " ++ show (Tag tm ty))
+  Right _ -> Left $ TypeError "Value can't be tagged with ADT"
+  Left _ -> Left $ TypeError "Elaboration Failed"
 infer ctx (Case tm cases) = inferMatch ctx (Case tm cases)
 infer ctx (BinOp (Arith _) e1 e2) =
-    infer ctx e1 >>= \t1 ->
-        infer ctx e2 >>= \t2 ->
-            if t1 == TyCInt && check ctx e2 TyCInt
-                then Right TyCInt
-                else Left $ TypeError ("Type mismatch in arithmetic operation " ++ show t1 ++ " " ++ show t2)
+  infer ctx e1 >>= \t1 ->
+    infer ctx e2 >>= \t2 ->
+      if t1 == TyCInt && check ctx e2 TyCInt
+        then Right TyCInt
+        else Left $ TypeError ("Type mismatch in arithmetic operation " ++ show t1 ++ " " ++ show t2)
 infer ctx (BinOp (Comp _) e1 e2) =
-    infer ctx e1 >>= \t1 ->
-        if check ctx e2 t1
-            then Right TyCBool
-            else
-                Left $
-                    TypeError "Type mismatch in comparison operation. Expected an integer, boolean, or string for comparison"
+  infer ctx e1 >>= \t1 ->
+    if check ctx e2 t1
+      then Right TyCBool
+      else
+        Left $
+          TypeError "Type mismatch in comparison operation. Expected an integer, boolean, or string for comparison"
 infer ctx (BinOp (Logic _) e1 e2) =
-    infer ctx e1 >>= \t1 ->
-        if t1 == TyCBool && check ctx e2 TyCBool
-            then Right TyCBool
-            else Left $ TypeError "Type mismatch in logical operation"
+  infer ctx e1 >>= \t1 ->
+    if t1 == TyCBool && check ctx e2 TyCBool
+      then Right TyCBool
+      else Left $ TypeError "Type mismatch in logical operation"
 infer ctx (UnOp Not e) =
-    if check ctx e TyCBool
-        then Right TyCBool
-        else Left $ TypeError "Expected boolean for negation"
-infer ctx (Nil ty) = Right ty
+  if check ctx e TyCBool
+    then Right TyCBool
+    else Left $ TypeError "Expected boolean for negation"
+infer _ (Nil ty) = Right $ TyCUnion TyCUnit ty
 infer ctx (Cons e1 e2) =
-    infer ctx e1 >>= \t1 ->
-        infer ctx e2 >>= \t2 ->
-            if TyCList t1 == t2
-                then Right $ TyCList t1
-                else Left $ TypeError ("List type check failed: " ++ "Expected type of list " ++ show t1 ++ ", but got " ++ show t2)
+  infer ctx e1 >>= \t1 ->
+    infer ctx e2
+      >>= \case
+        TyCUnion TyCUnit t2 ->
+          if t1 == t2
+            then Right $ TyCUnion TyCUnit t2
+            else Left $ TypeError "Type mismatch in Cons: head and tail types don't match."
+        _ -> Left $ TypeError "Second argument of Cons must be a list"
+
 infer ctx (LCase e1 e2 e3) = case infer ctx e1 of
-    Right (TyCList ty1) ->
-        infer ctx e2 >>= \ty2 ->
-            infer (TyCAnd (TyCAnd ctx ty1) (TyCList ty1)) e3 >>= \ty3 ->
-                if ty2 == ty3
-                    then Right $ TyCList ty1
-                    else Left $ TypeError "Case branches list pattern match don't have same types."
+  Right (TyCList ty1) ->
+    infer ctx e2 >>= \ty2 ->
+      infer (TyCAnd (TyCAnd ctx ty1) (TyCList ty1)) e3 >>= \ty3 ->
+        if ty2 == ty3
+          then Right $ TyCList ty1
+          else Left $ TypeError "Case branches list pattern match don't have same types."
 infer ctx (CLam ty tm) = Left $ TypeError "Linking not resolved properly"
 infer ctx (Anno tm ty) =
-    if check ctx tm ty
-        then Right ty
-        else Left $ TypeError "Types and Annotation don't match."
+  if check ctx tm ty
+    then Right ty
+    else Left $ TypeError "Types and Annotation don't match."
 infer _ _ = Left $ TypeError "Unknown expression"
 
 check :: CoreTyp -> CoreTm -> CoreTyp -> Bool
 check ctx e tA = case infer ctx e of
-    Right tB -> tA == tB
-    _ -> False
+  Right tB -> trace ("Inferred type: " ++ show tB ++ ", Expected type: " ++ show tA) $ tA == tB
+  _ -> False
